

# Cut-Cut Commutations Are Not Superfluous

Rémi Di Guardia  
Université Paris Cité, CNRS, IRIF, Paris, France  
diguardia@irif.fr

September 4, 2025

## Abstract

In the definition of a cut-elimination procedure, there often is a *cut* – *cut* commutation allowing to swap two *cut*-rules. This allows for instance to fully eliminate a chosen *cut*-rule without reducing other such rules in a proof. One may wonder whether such *cut* – *cut* steps are superfluous. We prove it is not the case in linear logic: some cut-free forms of a proof can only be reached using a *cut* – *cut* commutation.

## 1 Introduction

We consider the sequent calculus of linear logic [Gir87]. As many logics, it has a *cut*-rule and a rewriting system called *cut-elimination*, which details how to reach a cut-free (or normal) proof starting from a proof with possibly many *cut*-rules. Cut-elimination has been studied extensively in this system and more generally in linear logic (but mainly for its proof-net syntax): mostly its normalization [Acc13; DG99; LM08; Tor03; PT10] but also its confluence [CP05; Di24]. In particular, it is well-known one can reach a normal form without using any *cut* – *cut* commutations. One may wonder whether such *cut* – *cut* steps are superfluous: can the same normal forms be reached with and without *cut* – *cut* commutations? We answer this question negatively, exhibiting a simple counter-example. This counter-example is even one for the simpler multiplicative-exponential fragment of linear logic, that we will consider here for simplicity's sake.

## 2 Definitions

We define here the sequent calculus of multiplicative-exponential linear logic [Gir87], with its cut-elimination procedure. Formulas are given by the following grammar, where  $X$  is an atom in a given countable set:

$$A, B ::= X^+ \mid X^- \mid A \wp B \mid A \otimes B \mid \perp \mid 1 \mid ?A \mid !A$$

$$\begin{array}{c}
\frac{}{\vdash A^\perp, A} \text{ (ax)} \quad \frac{\vdash A^\perp, \Gamma \quad \vdash A, \Delta}{\vdash \Gamma, \Delta} \text{ (cut)} \\
\frac{\vdash A, B, \Gamma}{\vdash A \wp B, \Gamma} \text{ (\wp)} \quad \frac{\vdash A, \Gamma \quad \vdash B, \Delta}{\vdash A \otimes B, \Gamma, \Delta} \text{ (\otimes)} \quad \frac{\vdash \Gamma}{\vdash \perp, \Gamma} \text{ (\perp)} \quad \frac{}{\vdash 1} \text{ (1)} \\
\frac{\vdash A, \Gamma}{\vdash ?A, \Gamma} \text{ (?d)} \quad \frac{\vdash ?A, ?A, \Gamma}{\vdash ?A, \Gamma} \text{ (?c)} \quad \frac{\vdash \Gamma}{\vdash ?A, \Gamma} \text{ (?w)} \quad \frac{\vdash A, ?\Gamma}{\vdash !A, ?\Gamma} \text{ (!)}
\end{array}$$

Figure 1: Rules of Linear Logic

We define on formulas a function  $(\cdot)^\perp$  called **orthogonality**, also named negation or duality, through the following inductive definition:

$$\begin{array}{ll}
(X^+)^\perp = X^- & (X^-)^\perp = X^+ \\
(A \wp B)^\perp = B^\perp \otimes A^\perp & (A \otimes B)^\perp = B^\perp \wp A^\perp \\
\perp^\perp = 1 & 1^\perp = \perp \\
(?A)^\perp = !A^\perp & (!A)^\perp = ?A^\perp
\end{array}$$

Sequents are multisets of formulas written in the form  $\vdash A_1, \dots, A_n$ . Rules of linear logic are given on Fig. 1, where  $A$  and  $B$  stand for arbitrary formulas,  $\Gamma$  and  $\Delta$  for multisets of formulas. The notation  $? \Gamma$  means that each formula of  $\Gamma$  is a  $?$ -formula.

As in many systems with a *cut*-rule, the *cut*-rule is *admissible* in linear logic: the same sequents can be proved with and without the *cut*-rule. The procedure turning a proof into a *cut*-free one is called *cut-elimination*. As we will not use *ax*-  $\otimes$ -  $\wp$ - and  $?_c$ -formulas and rules, we give this rewriting system without them. For a full description, see [Di24, Chapter 1].

**Definition 1. Cut-elimination** is the rewriting system whose rules are described on Table 1, up to commuting the two branches of any *cut*-rule.

The up to commutation means one should also consider a version of each rule with the left and right premises of any *cut*-rule swapped. In particular, for the *cut* – *cut* case, there are in fact 4 rewriting rules.

In the  $?w - !$  case, the doubled  $?_w$ -rule means we apply a  $?_w$ -rule on each formula of  $? \Delta$ . The order in which these rules are applied has no importance; in other words, the  $?w - !$  step is non-deterministic according to the order in which the  $?_w$ -rules are applied.

### 3 Cut-cut commutations allow to reach more normal forms

One may wonder whether the same normal forms can be reached with and without *cut* – *cut* steps. This is not the case in multiplicative-exponential linear logic, and thus in linear logic in general.

$\perp - 1$	$\frac{\frac{\pi}{\vdash \Gamma} \quad \frac{(\perp) \quad \vdash 1}{\vdash 1} \quad (1)}{\vdash \Gamma} \quad (cut) \quad \xrightarrow{\beta} \quad \frac{\pi}{\vdash \Gamma}$
$?d - !$	$\frac{\frac{\pi}{\vdash A^\perp, \Gamma} \quad (?d) \quad \frac{\phi}{\vdash A, ?\Delta} \quad (!)}{\vdash \Gamma, ?\Delta} \quad (cut) \quad \xrightarrow{\beta} \quad \frac{\pi}{\vdash A^\perp, \Gamma} \quad \frac{\phi}{\vdash A, ?\Delta} \quad (cut)}{\vdash \Gamma, ?\Delta}$
$?w - !$	$\frac{\frac{\pi}{\vdash \Gamma} \quad (?w) \quad \frac{\phi}{\vdash A, ?\Delta} \quad (!)}{\vdash \Gamma, ?\Delta} \quad (cut) \quad \xrightarrow{\beta} \quad \frac{\pi}{\vdash \Gamma, ?\Delta} \quad (?w)$
$\perp - cut$	$\frac{\frac{\pi}{\vdash A^\perp, \Gamma} \quad (\perp) \quad \frac{\phi}{\vdash A, \Delta} \quad (cut)}{\vdash \perp, \Gamma, \Delta} \quad \xrightarrow{\beta} \quad \frac{\pi}{\vdash A^\perp, \Gamma} \quad \frac{\phi}{\vdash A, \Delta} \quad (cut)}{\vdash \perp, \Gamma, \Delta} \quad (\perp)$
$?d - cut$	$\frac{\frac{\pi}{\vdash A^\perp, B, \Gamma} \quad (?d) \quad \frac{\phi}{\vdash A, \Delta} \quad (cut)}{\vdash ?B, \Gamma, \Delta} \quad \xrightarrow{\beta} \quad \frac{\pi}{\vdash A^\perp, B, \Gamma} \quad \frac{\phi}{\vdash A, \Delta} \quad (cut)}{\vdash ?B, \Gamma, \Delta} \quad (?d)$
$?w - cut$	$\frac{\frac{\pi}{\vdash A^\perp, \Gamma} \quad (?w) \quad \frac{\phi}{\vdash A, \Delta} \quad (cut)}{\vdash ?B, \Gamma, \Delta} \quad \xrightarrow{\beta} \quad \frac{\pi}{\vdash A^\perp, \Gamma} \quad \frac{\phi}{\vdash A, \Delta} \quad (cut)}{\vdash ?B, \Gamma, \Delta} \quad (?w)$
$! - cut$	$\frac{\frac{\pi}{\vdash ?A^\perp, B, ?\Gamma} \quad (!) \quad \frac{\phi}{\vdash A, ?\Delta} \quad (!)}{\vdash !B, ?\Gamma, ?\Delta} \quad (cut) \quad \xrightarrow{\beta} \quad \frac{\pi}{\vdash ?A^\perp, B, ?\Gamma} \quad \frac{\phi}{\vdash A, ?\Delta} \quad (!)}{\vdash !B, ?\Gamma, ?\Delta} \quad (cut)}$
$cut - cut$	$\frac{\frac{\pi}{\vdash A^\perp, B^\perp, \Gamma} \quad \frac{\phi}{\vdash A, \Delta} \quad (cut) \quad \frac{\tau}{\vdash B, \Sigma} \quad (cut)}{\vdash \Gamma, \Delta, \Sigma} \quad \xrightarrow{\beta} \quad \frac{\pi}{\vdash A^\perp, B^\perp, \Gamma} \quad \frac{\tau}{\vdash B, \Sigma} \quad (cut)}{\vdash A^\perp, \Gamma, \Sigma} \quad \frac{\phi}{\vdash A, \Delta} \quad (cut)}{\vdash \Gamma, \Delta, \Sigma}$

Table 1: Cut-elimination –  $\perp$ ,  $1$ ,  $?d$ ,  $?w$  and  $!$  cases

**Lemma 2.** *There exist a proof  $\pi$  and a cut-free proof  $\phi$  such that  $\pi$  reduces by cut-elimination to  $\phi$  using a cut – cut elimination step, but  $\pi$  does not reduce to  $\phi$  without using a cut – cut elimination step.*

*Proof.* Set  $\pi$  the following proof:

$$\begin{array}{c}
\frac{\frac{\frac{\overline{\vdash 1} \quad (1)}{\vdash 1, \perp_c} \quad (\perp)}{\vdash 1, ?\perp_c} \quad (?_d) \quad \frac{\frac{\frac{\overline{\vdash 1_d} \quad (1)}{\vdash !1_d} \quad (!)}{\vdash !1_d, \perp_a} \quad (\perp)}{\vdash !1_c, \perp_a, ?\perp_b} \quad (cut)}{\vdash 1, \perp_a, ?\perp_b} \quad (cut)
\end{array}$$

We add letters as indices on  $\perp$ - and  $!$ -formulas to distinguish occurrences, and to make apparent that the upper *cut*-rule introduces formulas  $!1_d$  and  $?\perp_d$  while the bottom one introduces  $?\perp_c$  and  $!1_c$ .

Without *cut – cut* steps, cut-elimination on  $\pi$  leads to a unique normal form:

$$\begin{array}{c}
\frac{\frac{\overline{\vdash 1} \quad (1)}{\vdash 1, ?\perp_b} \quad (?_w)}{\vdash 1, \perp_a, ?\perp_b} \quad (\perp)
\end{array}$$

For our purpose, it is enough to prove any normal form reached without a *cut – cut* step has a  $\perp$ -rule at its root. This is the case: one first has to apply a  $\perp$  – *cut* step on the upper *cut*-rule; then, whatever happens on the upper *cut*-rule, the first step involving the bottom *cut*-rule must be a  $\perp$  – *cut* step, resulting in a  $\perp$ -rule at the root of the proof.

Meanwhile, consider the result of applying a *cut – cut* step first:

$$\begin{array}{c}
\frac{\frac{\frac{\overline{\vdash 1_d} \quad (1)}{\vdash !1_d} \quad (!) \quad \frac{\frac{\overline{\vdash 1} \quad (1)}{\vdash 1, \perp_c} \quad (\perp)}{\vdash 1, ?\perp_c} \quad (?_d)}{\vdash !1_d, \perp_a} \quad (\perp) \quad \frac{\frac{\frac{\overline{\vdash 1} \quad (1)}{\vdash 1} \quad (1)}{\vdash ?\perp_d, 1_c} \quad (?_w)}{\vdash ?\perp_d, !1_c, ?\perp_b} \quad (!)}{\vdash ?\perp_d, 1, ?\perp_b} \quad (cut)}{\vdash 1, \perp_a, ?\perp_b} \quad (cut)
\end{array}$$

Here, one can apply a  $?\perp_d - !$  step on the upper *cut*-rule, then a  $?\perp_w - cut$  step still on this *cut*-rule, followed by a  $?\perp_w - cut$  step on the bottom *cut*-rule, leading to a proof with a  $?\perp_w$ -rule at its root. In particular, one can reach the following normal form  $\phi$ :

$$\begin{array}{c}
\frac{\frac{\overline{\vdash 1} \quad (1)}{\vdash 1, \perp_a} \quad (\perp)}{\vdash 1, \perp_a, ?\perp_b} \quad (?_w)
\end{array}$$

□

## 4 Conclusion

Perhaps surprisingly, *cut* – *cut* commutative steps of cut-elimination have a computational content: they allow to reach more normal forms in multiplicative-exponential linear logic, and so in linear logic. Nonetheless, our example seems hard to adapt without a contextual rule such as  $!$  – which needs the sequent it is applied on to be of the shape  $!A, ?\Gamma$ . Hence, we conjecture that in the multiplicative-additive fragment of linear logic the same normal forms can be reached with and without *cut* – *cut* commutative steps.

## References

- [Acc13] Beniamino Accattoli. “Linear Logic and Strong Normalization”. In: *Rewriting Techniques and Applications*. Ed. by Femke van Raamsdonk. Vol. 21. Leibniz International Proceedings in Informatics (LIPIcs). Schloss Dagstuhl – Leibniz-Zentrum für Informatik, 2013, pp. 39–54. DOI: 10.4230/LIPIcs.RTA.2013.39.
- [CP05] Robin Cockett and Craig Pastro. “A Language For Multiplicative-additive Linear Logic”. In: *Electronic Notes in Theoretical Computer Science* 122 (2005). Proceedings of the 10th Conference on Category Theory in Computer Science (CTCS 2004), pp. 23–65. DOI: /10.1016/j.entcs.2004.06.049. URL: <https://www.sciencedirect.com/science/article/pii/S1571066105000320>.
- [DG99] Roberto Di Cosmo and Stefano Guerrini. “Strong Normalization of Proof Nets Modulo Structural Congruences”. In: *Rewriting Techniques and Applications*. Ed. by P. Narendran and M. Rusinowitch. Vol. 1631. Lecture Notes in Computer Science. Springer, 1999, pp. 75–89. DOI: 10.1007/3-540-48685-2\_6.
- [Di24] Rémi Di Guardia. “Identity of Proofs and Formulas using Proof-Nets in Multiplicative-Additive Linear Logic”. Thèse de Doctorat. Ecole normale supérieure de lyon - ENS LYON, Sept. 2024. URL: <https://theses.hal.science/tel-04830060>.
- [Gir87] Jean-Yves Girard. “Linear logic”. In: *Theoretical Computer Science* 50 (1987), pp. 1–102. DOI: 10.1016/0304-3975(87)90045-4.
- [LM08] Olivier Laurent and Roberto Maieli. “Cut Elimination for Monomial MALL Proof Nets”. In: *Proceedings of the twenty-third annual symposium on Logic In Computer Science*. IEEE. IEEE Computer Society Press, June 2008, pp. 486–497.
- [PT10] Michele Pagani and Lorenzo Tortora de Falco. “Strong normalization property for second order linear logic”. In: *Theoretical Computer Science* 411.2 (2010), pp. 410–444.
- [Tor03] Lorenzo Tortora de Falco. “Additives of linear logic and normalization- Part I: a (restricted) Church-Rosser property”. In: *Theoretical Computer Science* 294.3 (Feb. 2003), pp. 489–524. DOI: 10.1016/S0304-3975(01)00176-1.